AczelSetTheory/CList/Filter.lean
@@ -1,3 +1,9 @@
+/-
+Copyright (c) 2026. All rights reserved.
+Author: Julián Calderón Almendros
+License: MIT
+-/
+
 import AczelSetTheory.CList.ExtEq
 
 namespace CList
@@ -7,38 +13,31 @@ def P_respects (P : CList → Bool) : Prop :=
   ∀ (x y : CList), extEq x y = true → P x = P y
 
 theorem subset_filter
-  (P : CList → Bool) (xs : List CList) :
-    subset (mk (xs.filter P)) (mk xs) = true
-      := by
+    (P : CList → Bool) (xs : PList CList) :
+    subset (mk (PList.filter P xs)) (mk xs) = true := by
   induction xs with
-  | nil => simp only [List.filter_nil, subset_nil]
+  | nil => exact subset_nil _
   | cons z zs ih =>
-    simp only [List.filter_cons]
+    simp only [PList.filter]
     split
     · simp only [subset_cons, Bool.and_eq_true]
-      have hz : mem z (mk (z :: zs)) = true := by
-        simp only [mem_cons, extEq_refl, Bool.true_or]
-      have hsub : subset (mk (zs.filter P)) (mk (z :: zs)) = true := by
-        exact subset_mono (zs.filter P) z zs ih
-      exact ⟨hz, hsub⟩
-    · exact subset_mono (zs.filter P) z zs ih
+      exact ⟨by simp only [mem_cons, extEq_refl, Bool.true_or], subset_mono (PList.filter P zs) z zs ih⟩
+    · exact subset_mono (PList.filter P zs) z zs ih
 
 theorem mem_filter_of_mem
-  (P : CList → Bool) (hP_resp : P_respects P) (x : CList) (xs : List CList)
-  (hx : mem x (mk xs) = true) (hPx : P x = true) :
-    mem x (mk (xs.filter P)) = true
-      := by
+    (P : CList → Bool) (hP_resp : P_respects P) (x : CList) (xs : PList CList)
+    (hx : mem x (mk xs) = true) (hPx : P x = true) :
+    mem x (mk (PList.filter P xs)) = true := by
   induction xs with
   | nil => simp [mem_nil] at hx
   | cons z zs ih =>
-    simp only [List.filter_cons]
-    simp only [mem_cons, Bool.or_eq_true] at hx ⊢
+    simp only [PList.filter]
+    simp only [mem_cons, Bool.or_eq_true] at hx
     cases hx with
     | inl heq =>
       have hzP : P z = true := by
         have : P z = P x := hP_resp z x (extEq_comm x z ▸ heq)
-        rw [this]
-        exact hPx
+        rw [this]; exact hPx
       simp only [hzP, ite_true, mem_cons, Bool.or_eq_true]
       exact Or.inl heq
     | inr hmem =>
@@ -49,20 +48,22 @@ theorem mem_filter_of_mem
       · exact hind
 
 theorem filter_subset_filter
-  (P : CList → Bool) (hP_resp : P_respects P) (xs ys : List CList)
-  (hsub : subset (mk xs) (mk ys) = true) :
-    subset (mk (xs.filter P)) (mk (ys.filter P)) = true
-      := by
+    (P : CList → Bool) (hP_resp : P_respects P) (xs ys : PList CList)
+    (hsub : subset (mk xs) (mk ys) = true) :
+    subset (mk (PList.filter P xs)) (mk (PList.filter P ys)) = true := by
   induction xs with
-  | nil => simp [List.filter_nil, subset_nil]
+  | nil => exact subset_nil _
   | cons z zs ih =>
-    simp only [List.filter_cons]
+    simp only [PList.filter]
     split
     · next hzP =>
       simp only [subset_cons, Bool.and_eq_true]
-      have hz_in_xs : mem z (mk (z :: zs)) = true := by simp only [mem_cons, extEq_refl, Bool.true_or]
-      have hz_in_ys : mem z (mk ys) = true := mem_subset z (mk (z :: zs)) (mk ys) hz_in_xs hsub
-      have hz_in_ys_filter : mem z (mk (ys.filter P)) = true := mem_filter_of_mem P hP_resp z ys hz_in_ys hzP
+      have hz_in_xs : mem z (mk (.cons z zs)) = true := by
+        simp only [mem_cons, extEq_refl, Bool.true_or]
+      have hz_in_ys : mem z (mk ys) = true :=
+        mem_subset z (mk (.cons z zs)) (mk ys) hz_in_xs hsub
+      have hz_in_ys_filter : mem z (mk (PList.filter P ys)) = true :=
+        mem_filter_of_mem P hP_resp z ys hz_in_ys hzP
       have hzs_sub_ys : subset (mk zs) (mk ys) = true := by
         simp only [subset_cons, Bool.and_eq_true] at hsub
         exact hsub.2
@@ -71,33 +72,29 @@ theorem filter_subset_filter
       exact ih hsub.2
 
 theorem extEq_filter
-  (P : CList → Bool) (hP_resp : P_respects P) (xs ys : List CList)
-  (heq : extEq (mk xs) (mk ys) = true) :
-    extEq (mk (xs.filter P)) (mk (ys.filter P)) = true
-      := by
+    (P : CList → Bool) (hP_resp : P_respects P) (xs ys : PList CList)
+    (heq : extEq (mk xs) (mk ys) = true) :
+    extEq (mk (PList.filter P xs)) (mk (PList.filter P ys)) = true := by
   simp only [extEq_def, Bool.and_eq_true] at heq ⊢
-  exact ⟨filter_subset_filter P hP_resp xs ys heq.1, filter_subset_filter P hP_resp ys xs heq.2⟩
-
+  exact ⟨filter_subset_filter P hP_resp xs ys heq.1,
+         filter_subset_filter P hP_resp ys xs heq.2⟩
 
 theorem P_of_mem_filter
-  (P : CList → Bool) (hP_resp : P_respects P) (x : CList) (xs : List CList)
-  (hx : mem x (mk (xs.filter P)) = true) :
-    P x = true
-      := by
+    (P : CList → Bool) (hP_resp : P_respects P) (x : CList) (xs : PList CList)
+    (hx : mem x (mk (PList.filter P xs)) = true) :
+    P x = true := by
   induction xs with
-  | nil => simp [mem_nil] at hx
+  | nil => simp [PList.filter, mem_nil] at hx
   | cons z zs ih =>
-    simp only [List.filter_cons] at hx
+    simp only [PList.filter] at hx
     split at hx
     · next hzP =>
       simp only [mem_cons, Bool.or_eq_true] at hx
       cases hx with
       | inl heq =>
         have h_px_pz : P x = P z := hP_resp x z heq
-        rw [h_px_pz]
-        exact hzP
-      | inr hmem =>
-        exact ih hmem
+        rw [h_px_pz]; exact hzP
+      | inr hmem => exact ih hmem
     · exact ih hx
 
 end CList
